explicit constructor for InputBuffer

src/3d/prelude/buffer/EverParse3d.InputStream.Buffer.Aux.fst
@@ -5,6 +5,8 @@ module EverParse3d.InputStream.Buffer.Aux
 module B = LowStar.Buffer
 module U8 = FStar.UInt8
 module U32 = FStar.UInt32
+module HS = FStar.HyperStack
+module HST = FStar.HyperStack.ST
 
 #set-options "--__temp_no_proj EverParse3d.InputStream.Buffer.Aux"
 
@@ -23,3 +25,70 @@ type input_buffer = {
     Ghost.reveal g_all == Seq.slice g_all_buf 0 (U32.v len)
   );
 }
+
+inline_for_extraction
+noextract
+let t = input_buffer
+
+unfold
+let _live
+  (x: t)
+  (h: HS.mem)
+: Tot prop
+=
+  B.live h x.buf /\
+  B.live h x.pos /\
+  U32.v (B.deref h x.pos) <= U32.v x.len /\
+  B.as_seq h x.buf == Ghost.reveal x.g_all_buf /\
+  Seq.slice (B.as_seq h x.buf) 0 (U32.v x.len) == Ghost.reveal x.g_all
+
+let _footprint
+  (x: t)
+: Ghost B.loc
+  (requires True)
+  (ensures (fun y -> B.address_liveness_insensitive_locs `B.loc_includes` y))
+= B.loc_buffer x.buf `B.loc_union` B.loc_buffer x.pos
+
+let _get_remaining
+  (x: t)
+  (h: HS.mem)
+: Ghost (Seq.seq U8.t)
+  (requires (_live x h))
+  (ensures (fun y -> Seq.length y <= U32.v x.len))
+= 
+  let i = U32.v (B.deref h x.pos) in
+  Seq.slice x.g_all i (Seq.length x.g_all)
+
+val make_input_buffer
+  (from: B.buffer U8.t)
+  (n: U32.t)
+  (pos: B.pointer U32.t)
+: HST.Stack t
+  (requires (fun h ->
+    B.live h from /\
+    B.live h pos /\
+    B.loc_disjoint (B.loc_buffer from) (B.loc_buffer pos) /\
+    U32.v n == B.length from
+  ))
+  (ensures (fun h res h' ->
+    B.modifies (B.loc_buffer from `B.loc_union` B.loc_buffer pos) h h' /\
+    _footprint res `B.loc_includes` (B.loc_buffer from `B.loc_union` B.loc_buffer pos) /\
+    (B.loc_buffer from `B.loc_union` B.loc_buffer pos) `B.loc_includes` _footprint res /\
+    _live res h' /\
+    _get_remaining res h' == B.as_seq h from
+  ))
+
+open LowStar.BufferOps
+
+let make_input_buffer from n pos =
+  let h = HST.get () in
+  let g = Ghost.hide (B.as_seq h from) in
+  pos *= 0ul;
+  {
+    buf = from;
+    len = n;
+    pos = pos;
+    g_all = g;
+    g_all_buf = g;
+    prf = ();
+  }
